progress on ZFC in classical alpha set

alpha_set_classical.v
@@ -1072,4 +1072,774 @@ Qed.
 End EuclidPrimesKeyLemmas.
 
 
-(* TODO: ZFC foundation recovery *)
+Section ZFC_in_ClassicalAlpha.
+Context `{H_alpha: ClassicalAlphaSet}.
+
+(* Sets are just predicates - rename to avoid conflict with Coq's Set *)
+Definition ZSet := AlphaPred.
+
+(* Membership is predicate application *)
+Definition In (x : Alphacarrier) (A : ZSet) : Prop := A x.
+Notation "x 'in' A" := (In x A) (at level 70).
+Notation "x 'notin' A" := (~ In x A) (at level 70).
+
+(* Set equality via extensionality *)
+Definition set_eq (A B : ZSet) : Prop := pred_equiv A B.
+Notation "A == B" := (set_eq A B) (at level 70).
+
+(* Axiom 1: Extensionality (but it's just pred_equiv!) *)
+Theorem extensionality : forall A B : ZSet,
+  (forall x, x in A <-> x in B) <-> A == B.
+Proof.
+  intros A B.
+  unfold set_eq, pred_equiv, In.
+  split; intro H; exact H.
+Qed.
+
+(* Axiom 2: Empty Set (it's the_impossible!) *)
+Definition Empty : ZSet := the_impossible.
+
+Theorem empty_set_exists : exists E : ZSet, forall x, x notin E.
+Proof.
+  exists Empty.
+  intros x.
+  unfold In, Empty.
+  apply the_impossible_is_impossible.
+Qed.
+
+(* Singleton sets *)
+Definition singleton (a : Alphacarrier) : ZSet :=
+  fun x => x = a.
+
+Theorem singleton_spec : forall a x,
+  x in singleton a <-> x = a.
+Proof.
+  intros a x.
+  unfold In, singleton.
+  split; intro H; exact H.
+Qed.
+
+(* Now let's try pairing *)
+Definition pair (a b : Alphacarrier) : ZSet :=
+  fun x => x = a \/ x = b.
+
+Theorem pair_spec : forall a b x,
+  x in pair a b <-> (x = a \/ x = b).
+Proof.
+  intros a b x.
+  unfold In, pair.
+  split; intro H; exact H.
+Qed.
+
+
+(* Prove singletons are not empty (when element exists) *)
+Theorem singleton_not_empty : forall a,
+ ~ (singleton a == Empty).
+Proof.
+ intros a H_eq.
+ (* If singleton a == Empty, then a in singleton a <-> a in Empty *)
+ assert (a in singleton a) by (apply singleton_spec; reflexivity).
+ assert (a in Empty) by (apply H_eq; exact H).
+ (* But nothing is in Empty *)
+ unfold In, Empty in H0.
+ apply (the_impossible_is_impossible a).
+ exact H0.
+Qed.
+
+(* Prove pairs are not empty *)
+Theorem pair_not_empty : forall a b,
+ ~ (pair a b == Empty).
+Proof.
+ intros a b H_eq.
+ assert (a in pair a b) by (apply pair_spec; left; reflexivity).
+ assert (a in Empty) by (apply H_eq; exact H).
+ unfold In, Empty in H0.
+ apply (the_impossible_is_impossible a).
+ exact H0.
+Qed.
+
+(* Axiom 3: Pairing - we can form pairs! *)
+Theorem pairing_axiom : forall a b,
+ exists P : ZSet, forall x, x in P <-> (x = a \/ x = b).
+Proof.
+ intros a b.
+ exists (pair a b).
+ intro x.
+ apply pair_spec.
+Qed.
+
+(* Define subset relation *)
+Definition subset (A B : ZSet) : Prop :=
+ forall x, x in A -> x in B.
+Notation "A 'subseteq' B" := (subset A B) (at level 70).
+
+(* Binary union *)
+Definition union2 (A B : ZSet) : ZSet :=
+ fun x => x in A \/ x in B.
+
+Theorem union2_spec : forall A B x,
+ x in union2 A B <-> (x in A \/ x in B).
+Proof.
+ intros A B x.
+ unfold In, union2.
+ split; intro H; exact H.
+Qed.
+
+(* Intersection *)
+Definition inter2 (A B : ZSet) : ZSet :=
+ fun x => x in A /\ x in B.
+
+Theorem inter2_spec : forall A B x,
+ x in inter2 A B <-> (x in A /\ x in B).
+Proof.
+ intros A B x.
+ unfold In, inter2.
+ split; intro H; exact H.
+Qed.
+
+(* Set difference *)
+Definition diff (A B : ZSet) : ZSet :=
+ fun x => x in A /\ x notin B.
+
+Theorem diff_spec : forall A B x,
+ x in diff A B <-> (x in A /\ x notin B).
+Proof.
+ intros A B x.
+ unfold In, diff.
+ split; intro H; exact H.
+Qed.
+
+(* Complement (relative to universal set) *)
+Definition compl (A : ZSet) : ZSet :=
+ fun x => x notin A.
+
+(* The universal set is the_necessary! *)
+Definition Universal : ZSet := the_necessary.
+
+Theorem universal_contains_all : forall x,
+ x in Universal.
+Proof.
+ intros x.
+ unfold In, Universal, the_necessary.
+ apply the_impossible_is_impossible.
+Qed.
+
+(* Basic set algebra theorems *)
+Theorem union_empty_left : forall A,
+ union2 Empty A == A.
+Proof.
+ intros A.
+ unfold set_eq, pred_equiv.
+ intros x.
+ split.
+ - intros [H_empty | H_A].
+   + (* x in Empty - impossible *)
+     unfold In, Empty in H_empty.
+     exfalso.
+     apply (the_impossible_is_impossible x).
+     exact H_empty.
+   + exact H_A.
+ - intros H_A.
+   right. exact H_A.
+Qed.
+
+Theorem inter_empty_left : forall A,
+ inter2 Empty A == Empty.
+Proof.
+ intros A.
+ unfold set_eq, pred_equiv.
+ intros x.
+ split.
+ - intros [H_empty H_A].
+   exact H_empty.
+ - intros H_empty.
+   split.
+   + exact H_empty.
+   + (* Need to show x in A, but we know x in Empty which is impossible *)
+     unfold In, Empty in H_empty.
+     exfalso.
+     apply (the_impossible_is_impossible x).
+     exact H_empty.
+Qed.
+
+(* De Morgan's laws for sets *)
+Theorem de_morgan_union : forall A B,
+  compl (union2 A B) == inter2 (compl A) (compl B).
+Proof.
+  intros A B.
+  unfold set_eq, pred_equiv.
+  intros x.
+  unfold In, compl, union2, inter2.
+  (* Now we have: ~ (A x \/ B x) <-> ~ A x /\ ~ B x *)
+  split.
+  - (* Forward direction *)
+    intros H_not_union.
+    split.
+    + intros H_A. 
+      apply H_not_union.
+      left. exact H_A.
+    + intros H_B.
+      apply H_not_union.
+      right. exact H_B.
+  - (* Backward direction *)
+    intros [H_not_A H_not_B] [H_A | H_B].
+    + exact (H_not_A H_A).
+    + exact (H_not_B H_B).
+Qed.
+
+Theorem de_morgan_inter : forall A B,
+  compl (inter2 A B) == union2 (compl A) (compl B).
+Proof.
+  intros A B.
+  unfold set_eq, pred_equiv.
+  intros x.
+  unfold In, compl, inter2, union2.
+  (* Now we have: ~ (A x /\ B x) <-> ~ A x \/ ~ B x *)
+  split.
+  - (* Forward direction - need classical logic here *)
+    intros H_not_inter.
+    destruct (alpha_constant_decision (A x)) as [H_A | H_not_A].
+    + (* If A x, then must have ~ B x *)
+      right.
+      intros H_B.
+      apply H_not_inter.
+      split; assumption.
+    + (* If ~ A x, we're done *)
+      left. exact H_not_A.
+  - (* Backward direction *)
+    intros [H_not_A | H_not_B] [H_A H_B].
+    + exact (H_not_A H_A).
+    + exact (H_not_B H_B).
+Qed.
+
+
+(* Axiomatize that some elements of Alphacarrier can represent sets *)
+(* This is like saying "some elements are sets" in ZFC *)
+Axiom is_set_code : Alphacarrier -> Prop.
+Axiom set_decode : Alphacarrier -> ZSet.
+
+(* set_decode is only meaningful for set codes *)
+Axiom decode_only_codes : forall x,
+  ~ is_set_code x -> set_decode x == Empty.
+
+(* For any predicate that's "set-like", there's a code for it *)
+Axiom set_encode_exists : forall (S : ZSet), 
+  (exists a, S a) \/ (forall a, ~ S a) ->  (* S is not "middle" *)
+  exists x, is_set_code x /\ set_decode x == S.
+
+(* The membership relation for coded sets *)
+Definition mem (a b : Alphacarrier) : Prop :=
+  is_set_code b /\ a in set_decode b.
+
+Notation "a 'mem' b" := (mem a b) (at level 70).
+
+(* Let's verify this works with basic examples *)
+Theorem empty_set_has_code : 
+  exists e, is_set_code e /\ set_decode e == Empty.
+Proof.
+  apply set_encode_exists.
+  right. intros a H.
+  unfold Empty, In, the_impossible in H.
+  apply (the_impossible_is_impossible a H).
+Qed.
+
+(* Basic theorems about set codes *)
+Theorem singleton_has_code : forall a,
+  exists s, is_set_code s /\ set_decode s == singleton a.
+Proof.
+  intro a.
+  apply set_encode_exists.
+  left. exists a. 
+  unfold singleton, In. reflexivity.
+Qed.
+
+Theorem pair_has_code : forall a b,
+  exists p, is_set_code p /\ set_decode p == pair a b.
+Proof.
+  intros a b.
+  apply set_encode_exists.
+  left. exists a.
+  unfold pair, In. left. reflexivity.
+Qed.
+
+(* Union axiom - for any set of sets, their union exists *)
+Definition is_union_of (F union_set : Alphacarrier) : Prop :=
+  is_set_code F /\ is_set_code union_set /\
+  forall x, x mem union_set <-> exists Y, Y mem F /\ x mem Y.
+
+Axiom union_exists : forall F,
+  is_set_code F ->
+  exists U, is_union_of F U.
+
+
+(* Binary union as a special case *)
+Theorem binary_union_exists : forall A B,
+  is_set_code A -> is_set_code B ->
+  exists U, is_set_code U /\ 
+    forall x, x mem U <-> (x mem A \/ x mem B).
+Proof.
+  intros A B HA HB.
+  (* First, create a pair {A, B} *)
+  destruct (pair_has_code A B) as [P [HP HPdecode]].
+  (* Then take union of this pair *)
+  destruct (union_exists P HP) as [U HU].
+  exists U.
+  destruct HU as [HF [HUcode HUspec]].
+  split; [exact HUcode|].
+  intro x.
+  split.
+  - intro HxU.
+    apply HUspec in HxU.
+    destruct HxU as [Y [HYP HxY]].
+    (* Y mem P means is_set_code P /\ Y in set_decode P *)
+    destruct HYP as [_ HYP'].
+    (* Use HPdecode as a function *)
+    assert (Y in pair A B).
+    { apply HPdecode. exact HYP'. }
+    apply pair_spec in H.
+    destruct H as [HYA | HYB].
+    + left. subst Y. exact HxY.
+    + right. subst Y. exact HxY.
+  - intros [HxA | HxB].
+    + apply HUspec.
+      exists A. split; [|exact HxA].
+      split; [exact HP|].
+      (* Again, use HPdecode as a function *)
+      apply HPdecode.
+      apply pair_spec. left. reflexivity.
+    + apply HUspec.
+      exists B. split; [|exact HxB].
+      split; [exact HP|].
+      apply HPdecode.
+      apply pair_spec. right. reflexivity.
+Qed.
+
+(* Separation axiom schema - for any set and property, we can form the subset *)
+Axiom separation : forall A (P : Alphacarrier -> Prop),
+  is_set_code A ->
+  exists B, is_set_code B /\
+    forall x, x mem B <-> (x mem A /\ P x).
+
+(* Example: intersection via separation *)
+Theorem intersection_exists : forall A B,
+  is_set_code A -> is_set_code B ->
+  exists I, is_set_code I /\
+    forall x, x mem I <-> (x mem A /\ x mem B).
+Proof.
+  intros A B HA HB.
+  apply (separation A (fun x => x mem B) HA).
+Qed.
+
+
+(* First, let's define the successor operation in set theory *)
+(* Successor of x is x union {x} *)
+Definition is_successor (x sx : Alphacarrier) : Prop :=
+  is_set_code x /\ is_set_code sx /\
+  forall y, y mem sx <-> (y mem x \/ y = x).
+
+(* The axiom of infinity: there exists an inductive set *)
+(* A set is inductive if it contains empty and is closed under successor *)
+Definition is_inductive (I : Alphacarrier) : Prop :=
+  is_set_code I /\
+  (exists e, is_set_code e /\ (forall x, ~ (x mem e)) /\ e mem I) /\  (* contains empty *)
+  (forall x, x mem I -> exists sx, is_successor x sx /\ sx mem I).      (* closed under successor *)
+
+Axiom infinity : exists I, is_inductive I.
+
+(* Direct axiomatization of important set codes *)
+Axiom empty_code : Alphacarrier.
+Axiom empty_code_spec : is_set_code empty_code /\ set_decode empty_code == Empty.
+
+(* Similarly for other constructions *)
+Axiom singleton_code : Alphacarrier -> Alphacarrier.
+Axiom singleton_code_spec : forall a,
+  is_set_code (singleton_code a) /\ 
+  set_decode (singleton_code a) == singleton a.
+
+Axiom pair_code : Alphacarrier -> Alphacarrier -> Alphacarrier.
+Axiom pair_code_spec : forall a b,
+  is_set_code (pair_code a b) /\ 
+  set_decode (pair_code a b) == pair a b.
+
+Axiom successor_code : Alphacarrier -> Alphacarrier.
+Axiom successor_code_spec : forall x,
+  is_set_code x -> is_successor x (successor_code x).
+
+(* Alternative approach - let's make a cleaner lemma first *)
+Lemma not_mem_empty : forall x, ~ (x mem empty_code).
+Proof.
+  intros x [Hcode Hin].
+  destruct empty_code_spec as [_ Hdecode].
+  apply Hdecode in Hin.
+  unfold In, Empty in Hin.
+  exact (the_impossible_is_impossible x Hin).
+Qed.
+
+(* Now the theorem is trivial *)
+Theorem zero_exists_zfc : exists z,
+  is_set_code z /\ forall x, ~ (x mem z).
+Proof.
+  exists empty_code.
+  destruct empty_code_spec as [Hcode _].
+  split.
+  - exact Hcode.
+  - exact not_mem_empty.
+Qed.
+
+(* Let's build the first few natural numbers explicitly *)
+Definition zero_zfc := empty_code.
+Definition one_zfc := successor_code zero_zfc.
+Definition two_zfc := successor_code one_zfc.
+Definition three_zfc := successor_code two_zfc.
+
+(* Prove basic properties *)
+Lemma zero_is_empty : forall x, ~ (x mem zero_zfc).
+Proof.
+  exact not_mem_empty.
+Qed.
+
+Lemma one_contains_only_zero : forall x,
+  x mem one_zfc <-> x = zero_zfc.
+Proof.
+  intro x.
+  unfold one_zfc.
+  destruct empty_code_spec as [Hcode _].
+  destruct (successor_code_spec zero_zfc Hcode) as [_ [Hscode Hspec]].
+  split.
+  - intro Hmem.
+    apply Hspec in Hmem.
+    destruct Hmem as [Hcontra | Heq].
+    + exfalso. exact (zero_is_empty x Hcontra).
+    + exact Heq.
+  - intro Heq.
+    subst x.
+    apply Hspec.
+    right. reflexivity.
+Qed.
+
+Lemma two_contains_zero_and_one : forall x,
+  x mem two_zfc <-> (x = zero_zfc \/ x = one_zfc).
+Proof.
+  intro x.
+  unfold two_zfc, one_zfc.
+  (* Get the properties of successor_code *)
+  destruct empty_code_spec as [Hcode0 _].
+  
+  (* First application of successor_code_spec *)
+  assert (Hsucc1 := successor_code_spec zero_zfc Hcode0).
+  destruct Hsucc1 as [_ [Hcode_one Hspec1]].
+  (* Now Hcode_one : is_set_code (successor_code zero_zfc) *)
+  
+  (* Second application of successor_code_spec *)
+  assert (Hsucc2 := successor_code_spec (successor_code zero_zfc) Hcode_one).
+  destruct Hsucc2 as [_ [Hcode_two Hspec2]].
+  
+  split.
+  - intro Hmem.
+    apply Hspec2 in Hmem.
+    destruct Hmem as [Hin1 | Heq1].
+    + (* x mem one_zfc *)
+      apply one_contains_only_zero in Hin1.
+      left. exact Hin1.
+    + (* x = one_zfc *)
+      right. exact Heq1.
+  - intros [Hz | Ho].
+    + (* x = zero_zfc *)
+      subst x.
+      apply Hspec2.
+      left.
+      apply one_contains_only_zero.
+      reflexivity.
+    + (* x = one_zfc *)
+      subst x.
+      apply Hspec2.
+      right. reflexivity.
+Qed.
+
+(* Axiom: empty sets have unique codes *)
+Axiom empty_unique : forall e1 e2,
+  is_set_code e1 -> is_set_code e2 ->
+  (forall x, ~ (x mem e1)) ->
+  (forall x, ~ (x mem e2)) ->
+  e1 = e2.
+
+(* The natural numbers are the intersection of all inductive sets *)
+Definition is_natural_number (n : Alphacarrier) : Prop :=
+  forall I, is_inductive I -> n mem I.
+
+Theorem zero_is_natural : is_natural_number zero_zfc.
+Proof.
+  unfold is_natural_number, zero_zfc.
+  intros I HI.
+  destruct HI as [HIcode [[e [He [Hemp Hemem]]] Hclosed]].
+  (* Both empty_code and e are empty sets *)
+  assert (e = empty_code).
+  { apply empty_unique.
+    - exact He.
+    - destruct empty_code_spec; assumption.
+    - exact Hemp.
+    - exact not_mem_empty. }
+  subst e.
+  exact Hemem.
+Qed.
+
+(* Supporting axioms we need for natural numbers *)
+Axiom nat_set_code : Alphacarrier.
+Axiom nat_set_code_spec : 
+  is_set_code nat_set_code /\
+  forall n, n mem nat_set_code <-> is_natural_number n.
+
+Axiom nat_is_set_code : forall n,
+  is_natural_number n -> is_set_code n.
+
+Axiom successor_preserves_nat : forall n,
+  is_natural_number n -> is_natural_number (successor_code n).
+
+(* Induction principle for natural numbers *)
+Theorem nat_induction_zfc : forall (P : Alphacarrier -> Prop),
+  P zero_zfc ->
+  (forall n, is_natural_number n -> P n -> P (successor_code n)) ->
+  forall n, is_natural_number n -> P n.
+Proof.
+  intros P Hz Hsucc n Hn.
+  
+  (* The subset of naturals satisfying P *)
+  destruct nat_set_code_spec as [Hnat_code Hnat_spec].
+  destruct (separation nat_set_code P Hnat_code) as [S [HS HSspec]].
+  
+  (* Claim: S is inductive *)
+  assert (His_ind: is_inductive S).
+  { unfold is_inductive.
+    split; [exact HS|].
+    split.
+    - (* S contains empty/zero *)
+      exists zero_zfc.
+      split; [|split].
+      + destruct empty_code_spec; assumption.
+      + exact zero_is_empty.
+      + apply HSspec. split.
+        * apply Hnat_spec. exact zero_is_natural.
+        * exact Hz.
+    - (* S is closed under successor *)
+      intros x HxS.
+      (* Extract the components without modifying HxS *)
+      assert (Hx_components: x mem nat_set_code /\ P x).
+      { apply HSspec. exact HxS. }
+      destruct Hx_components as [Hx_in_nat Px].
+      
+      assert (Hx_nat: is_natural_number x).
+      { apply Hnat_spec. exact Hx_in_nat. }
+      
+      assert (Hx_code: is_set_code x).
+      { apply nat_is_set_code. exact Hx_nat. }
+      
+      exists (successor_code x).
+      split.
+      + apply successor_code_spec. exact Hx_code.
+      + apply HSspec. split.
+        * apply Hnat_spec. 
+          apply successor_preserves_nat. exact Hx_nat.
+        * apply Hsucc.
+          -- exact Hx_nat.
+          -- exact Px. }
+  
+  (* Since n is natural, it's in S *)
+  assert (n_in_S: n mem S).
+  { unfold is_natural_number in Hn.
+    exact (Hn S His_ind). }
+  
+  (* Therefore P n holds *)
+  apply HSspec in n_in_S.
+  destruct n_in_S as [_ Pn].
+  exact Pn.
+Qed.
+
+(* First, let's properly handle subset encoding *)
+Definition encodes_subset (x : Alphacarrier) (A : Alphacarrier) : Prop :=
+  is_set_code x /\ is_set_code A /\
+  forall y, y mem x -> y mem A.
+
+(* Power set: collection of all subsets of A *)
+Definition is_powerset (A ps : Alphacarrier) : Prop :=
+  is_set_code A /\ is_set_code ps /\
+  forall x, x mem ps <-> encodes_subset x A.
+
+(* Power Set Axiom *)
+Axiom powerset_exists : forall A,
+  is_set_code A -> exists ps, is_powerset A ps.
+
+(* Let's prove some basic properties *)
+Theorem empty_in_every_powerset : forall A ps,
+  is_set_code A -> is_powerset A ps ->
+  empty_code mem ps.
+Proof.
+  intros A ps HA Hps.
+  destruct Hps as [_ [Hps_code Hps_spec]].
+  apply Hps_spec.
+  unfold encodes_subset.
+  destruct empty_code_spec as [He_code _].
+  split; [exact He_code|].
+  split; [exact HA|].
+  intros y Hy.
+  (* y mem empty_code is impossible *)
+  exfalso.
+  exact (not_mem_empty y Hy).
+Qed.
+
+Theorem set_in_own_powerset : forall A ps,
+  is_set_code A -> is_powerset A ps ->
+  A mem ps.
+Proof.
+  intros A ps HA Hps.
+  destruct Hps as [_ [Hps_code Hps_spec]].
+  apply Hps_spec.
+  unfold encodes_subset.
+  split; [exact HA|].
+  split; [exact HA|].
+  intros y Hy.
+  (* y mem A -> y mem A is trivial *)
+  exact Hy.
+Qed.
+
+(* Singleton subsets *)
+(* Singleton subsets *)
+Theorem singleton_in_powerset : forall A ps a,
+  is_set_code A -> is_powerset A ps -> a mem A ->
+  exists sa, is_set_code sa /\ sa mem ps /\
+    forall x, x mem sa <-> x = a.
+Proof.
+  intros A ps a HA Hps Ha.
+  (* Get singleton code *)
+  exists (singleton_code a).
+  destruct (singleton_code_spec a) as [Hsa_code Hsa_decode].
+  split; [exact Hsa_code|].
+  split.
+  - (* singleton a is in powerset *)
+    destruct Hps as [_ [_ Hps_spec]].
+    apply Hps_spec.
+    unfold encodes_subset.
+    split; [exact Hsa_code|].
+    split; [exact HA|].
+    intros x Hx.
+    (* If x mem singleton a, then x = a, so x mem A *)
+    destruct Hx as [_ Hx_in].
+    assert (x in singleton a).
+    { apply Hsa_decode. exact Hx_in. }
+    (* Use singleton spec to get x = a *)
+    assert (x = a).
+    { apply singleton_spec. exact H. }
+    (* Now rewrite using the equality *)
+    rewrite H0.
+    exact Ha.
+  - (* Characterization of singleton *)
+    intros x.
+    split.
+    + intro Hx.
+      destruct Hx as [_ Hx_in].
+      assert (x in singleton a).
+      { apply Hsa_decode. exact Hx_in. }
+      apply singleton_spec.
+      exact H.
+    + intro Heq.
+      rewrite Heq.  (* Use rewrite instead of subst *)
+      split; [exact Hsa_code|].
+      apply Hsa_decode.
+      apply singleton_spec.
+      reflexivity.
+Qed.
+
+
+(* Replacement Axiom *)
+
+(* A relation is functional if it maps each input to at most one output *)
+Definition is_functional (R : Alphacarrier -> Alphacarrier -> Prop) : Prop :=
+  forall x y z, R x y -> R x z -> y = z.
+
+(* Replacement: The image of a set under a functional relation is a set *)
+Axiom replacement : forall A (R : Alphacarrier -> Alphacarrier -> Prop),
+  is_set_code A ->
+  is_functional R ->
+  exists B, is_set_code B /\
+    forall y, y mem B <-> exists x, x mem A /\ R x y.
+
+(* Example application: Construct {f(x) | x ∈ A} for any function f *)
+Definition function_image (A : Alphacarrier) (f : Alphacarrier -> Alphacarrier) : Prop :=
+  is_set_code A ->
+  exists B, is_set_code B /\
+    forall y, y mem B <-> exists x, x mem A /\ y = f x.
+
+Theorem function_image_exists : forall A f,
+  is_set_code A ->
+  exists B, is_set_code B /\
+    forall y, y mem B <-> exists x, x mem A /\ y = f x.
+Proof.
+  intros A f HA.
+  (* Define the relation R(x,y) := y = f(x) *)
+  pose (R := fun x y => y = f x).
+  (* Show R is functional *)
+  assert (Hfunc: is_functional R).
+  { unfold is_functional, R.
+    intros x y z Hy Hz.
+    (* Hy : y = f x, Hz : z = f x, so y = z by transitivity *)
+    rewrite Hy.
+    symmetry.
+    exact Hz. }
+  (* Apply replacement *)
+  destruct (replacement A R HA Hfunc) as [B [HB HBspec]].
+  exists B. split; [exact HB|].
+  intros y. split.
+  - intro HyB.
+    apply HBspec in HyB.
+    destruct HyB as [x [HxA Hy]].
+    exists x. split; [exact HxA|].
+    unfold R in Hy. exact Hy.
+  - intros [x [HxA Heq]].
+    apply HBspec.
+    exists x. split; [exact HxA|].
+    unfold R. exact Heq.
+Qed.
+
+(* Foundation/Regularity Axiom *)
+(* Every non-empty set has an ∈-minimal element *)
+Axiom foundation : forall A,
+  is_set_code A ->
+  (exists x, x mem A) ->
+  exists x, x mem A /\ forall y, y mem x -> ~ (y mem A).
+
+(* This prevents things like x ∈ x or infinite chains x₀ ∈ x₁ ∈ x₂ ∈ ... *)
+Theorem no_set_contains_itself : forall x,
+  is_set_code x -> ~ (x mem x).
+Proof.
+  intros x Hx Hmem.
+  (* Apply foundation to {x} *)
+  destruct (singleton_code_spec x) as [Hs_code Hs_decode].
+  assert (exists y, y mem singleton_code x).
+  { exists x. 
+    (* Need to show x mem singleton_code x *)
+    (* By definition, mem requires is_set_code and membership *)
+    split.
+    - exact Hs_code.
+    - apply Hs_decode.
+      apply singleton_spec.
+      reflexivity. }
+  destruct (foundation (singleton_code x) Hs_code H) as [y [Hy Hmin]].
+  (* y must be x since singleton only contains x *)
+  assert (y = x).
+  { destruct Hy as [_ Hy_in].
+    apply Hs_decode in Hy_in.
+    apply singleton_spec in Hy_in.
+    exact Hy_in. }
+  subst y.
+  (* But then x is minimal, so nothing in x is in singleton x *)
+  (* In particular, x in x implies x in singleton x, contradiction *)
+  apply (Hmin x Hmem).
+  (* Again, build mem without unfold *)
+  split.
+  - exact Hs_code.
+  - apply Hs_decode. 
+    apply singleton_spec. 
+    reflexivity.
+Qed.
+
+
+End ZFC_in_ClassicalAlpha.
